Big addition in encode.v.
The tactic [encode] should now work on all base types.

theories/lang/encode.v
@@ -12,35 +12,141 @@ Class Encode (A : Type) :=
 
 Notation "# v" := (encode v) (at level 8, format "# v").
 
-(* A few typical instances. *)
+(* -------------------------------------------------------------------------- *)
+
+(* The tactic [encode] expects a goal of the form [v = encode x],
+   where typically [v] is a known value and [x] is a metavariable.
+   Finding a suitable instantiation of [x] amounts to inverting
+   the function [encode]. *)
+
+Create HintDb encode.
+
+Ltac encode :=
+  eauto with encode.
+
+Local Ltac solve_encode :=
+  intros; subst; eauto.
+
+(* -------------------------------------------------------------------------- *)
+
+(* Unit. *)
 
 Global Instance Encode_unit : Encode unit :=
   { encode := λ tt, VUnit }.
 
+Lemma solve_encode_unit x :
+  () = x →
+  VUnit = #x.
+Proof. solve_encode. Qed.
+
+Global Hint Resolve solve_encode_unit : encode.
+
+(* -------------------------------------------------------------------------- *)
+
+(* Booleans. *)
+
 Global Instance Encode_bool : Encode bool :=
   { encode := λ b, VBool b }.
+
+Lemma solve_encode_false b :
+  false = b →
+  VFalse = #b.
+Proof. solve_encode. Qed.
+
+Lemma solve_encode_true b :
+  true = b →
+  VTrue = #b.
+Proof. solve_encode. Qed.
+
+Global Hint Resolve solve_encode_false solve_encode_true : encode.
+
+(* -------------------------------------------------------------------------- *)
+
+(* Natural numbers. *)
 
 Global Instance Encode_nat : Encode nat :=
   { encode := λ n, VInt (int.repr (Z.of_nat n)) }.
 
+Lemma solve_encode_nat i n :
+  i = int.repr (Z.of_nat n) →
+  VInt i = #n.
+Proof. solve_encode. Qed.
+
+Global Hint Resolve solve_encode_nat : encode.
+
+(* -------------------------------------------------------------------------- *)
+
+(* Integer numbers. *)
+
 Global Instance Encode_Z : Encode Z :=
   { encode := λ n, VInt (int.repr n) }.
 
-Global Instance Encode_pair `{Encode A, Encode B} : Encode (A * B) :=
-  { encode :=
-      λ '(a, b), VPair (encode a) (encode b) }.
+Lemma solve_encode_int i z :
+  i = int.repr z →
+  VInt i = #z.
+Proof. solve_encode. Qed.
+
+Global Hint Resolve solve_encode_int : encode.
+
+(* This should help: *)
+
+Global Hint Resolve
+   int.neg_repr
+   int.add_repr_repr
+   int.sub_repr_repr
+   int.mul_repr_repr
+   int.divs_repr_repr
+   int.mods_repr_repr
+   int.eq_repr_repr
+   int.lt_repr_repr
+: encode.
+
+(* TODO add hints that help prove [representable z]. *)
+
+(* -------------------------------------------------------------------------- *)
+
+(* Options. *)
 
 Global Instance Encode_option `{Encode A} : Encode (option A) :=
   { encode :=
-      λ o, match o with None => VNone | Some v => VSome (encode v) end }.
+      λ o, match o with None => VNone | Some v => VSome #v end }.
+
+Lemma solve_encode_None `{Encode A} (o : option A) :
+  None = o →
+  VNone = #o.
+Proof. solve_encode. Qed.
+
+Lemma solve_encode_Some `{Encode A} v (o : option A) (x : A) :
+  Some x = o →
+  v = #x →
+  VSome v = #o.
+Proof. solve_encode. Qed.
+
+Global Hint Resolve solve_encode_None solve_encode_Some : encode.
+
+(* -------------------------------------------------------------------------- *)
+
+(* Values. *)
+
+(* This instance is needed, for instance, for memory locations. *)
 
 Global Instance Encode_val : Encode val :=
   { encode := λ v, v }.
 
+Lemma solve_encode_val v :
+  v = #v.
+Proof. solve_encode. Qed.
+
+Global Hint Resolve solve_encode_val : encode.
+
+(* -------------------------------------------------------------------------- *)
+
+(* Lists. *)
+
 Fixpoint encode_list `{Encode A} (xs : list A) :=
   match xs with
   | []      => vNil
-  | x :: xs => vCons (encode x) (encode_list xs)
+  | x :: xs => vCons #x (encode_list xs)
   end.
 
 Global Instance Encode_list `{Encode A} : Encode (list A) :=
@@ -48,7 +154,123 @@ Global Instance Encode_list `{Encode A} : Encode (list A) :=
 
 Lemma encode_list_is_encode `{Encode A} :
   ∀ (xs : list A),
-  encode_list xs = encode xs.
-Proof.
-  reflexivity.
-Qed.
+  encode_list xs = #xs.
+Proof. solve_encode. Qed.
+
+Lemma solve_encode_Nil `{Encode A} (xs : list A) :
+  [] = xs →
+  vNil = #xs.
+Proof. solve_encode. Qed.
+
+Lemma solve_encode_Cons `{Encode A} (xs : list A) x xs' v1 v2 :
+  x :: xs' = xs →
+  v1 = #x →
+  v2 = #xs' →
+  vCons v1 v2 = #xs.
+Proof. solve_encode. Qed.
+
+Global Hint Resolve
+  encode_list_is_encode
+  solve_encode_Nil solve_encode_Cons
+: encode.
+
+(* -------------------------------------------------------------------------- *)
+
+(* Pairs, or tuples of arity 2. *)
+
+Global Instance Encode_tuple2
+  `{Encode A, Encode B}
+  : Encode (A * B)
+  | 10 (* lower priority than tuple3 and tuple4 below *)
+:=
+  { encode := λ '(a, b), VPair #a #b }.
+
+Lemma solve_encode_tuple2
+  `{Encode A} `{Encode B}
+  (a : A) (b : B)
+  va vb
+  t :
+  (a, b) = t →
+  va = #a →
+  vb = #b →
+  VPair va vb = #t.
+Proof. solve_encode. Qed.
+
+(* The lemma [solve_encode_tuple2] has 12 arguments. *)
+
+(* We cannot let [eapply] apply this lemma, as Coq would make
+   incorrect choices of the types A, B. *)
+
+Global Hint Extern 1 (_ = _) =>
+  notypeclasses refine (@solve_encode_tuple2
+    _ _ _ _ _ _ _ _
+    _ _ _ _
+  )
+  : encode.
+
+(* -------------------------------------------------------------------------- *)
+
+(* Tuples of arity 3. *)
+
+Global Instance Encode_tuple3
+  `{Encode A} `{Encode B} `{Encode C}
+  : Encode (A * B * C)
+  | 5 (* higher priority than tuple2; lower priority than tuple3 *)
+:=
+  { encode := λ '(a, b, c), VTuple3 #a #b #c }.
+
+Lemma solve_encode_tuple3
+  `{Encode A} `{Encode B} `{Encode C}
+  (a : A) (b : B) (c : C)
+  va vb vc
+  t :
+  (a, b, c) = t →
+  va = #a →
+  vb = #b →
+  vc = #c →
+  VTuple3 va vb vc = #t.
+Proof. solve_encode. Qed.
+
+(* The lemma [solve_encode_tuple3] has 17 arguments. *)
+
+Global Hint Extern 1 (_ = _) =>
+  notypeclasses refine (@solve_encode_tuple3
+    _ _ _ _ _ _ _ _
+    _ _ _ _ _ _ _ _
+    _
+  )
+  : encode.
+
+(* -------------------------------------------------------------------------- *)
+
+(* Tuples of arity 4. *)
+
+Global Instance Encode_tuple4
+  `{Encode A} `{Encode B} `{Encode C} `{Encode D}
+  : Encode (A * B * C * D)
+  | 0 (* higher priority than tuple2 and tuple3 above *)
+:=
+  { encode := λ '(a, b, c, d), VTuple4 #a #b #c #d }.
+
+Lemma solve_encode_tuple4
+  `{Encode A} `{Encode B} `{Encode C} `{Encode D}
+  (a : A) (b : B) (c : C) (d : D)
+  va vb vc vd
+  t :
+  (a, b, c, d) = t →
+  va = #a →
+  vb = #b →
+  vc = #c →
+  vd = #d →
+  VTuple4 va vb vc vd = #t.
+Proof. solve_encode. Qed.
+
+(* The lemma [solve_encode_tuple4] has 22 arguments. *)
+
+Global Hint Extern 1 (_ = _) =>
+  notypeclasses refine (@solve_encode_tuple4
+    _ _ _ _ _ _ _ _
+    _ _ _ _ _ _ _ _
+    _ _ _ _ _ _
+  )
+  : encode.
